add bitfield insert opcode but not yet used nor translated

mppa_k1c/ExtValues.v
@@ -41,8 +41,11 @@ Definition bitfield_maskl stop start :=
 
 Definition insf stop start prev fld :=
   let mask := bitfield_mask stop start in
-  Val.or (Val.and prev (Val.notint mask))
-         (Val.and (Val.shl fld (Vint (Int.repr start))) mask).
+  if is_bitfield stop start
+  then
+    Val.or (Val.and prev (Val.notint mask))
+           (Val.and (Val.shl fld (Vint (Int.repr start))) mask)
+  else Vundef.
 
 Definition is_bitfieldl stop start :=
   (Z.leb start stop)
@@ -74,5 +77,8 @@ Definition extfsl stop start v :=
 
 Definition insfl stop start prev fld :=
   let mask := bitfield_maskl stop start in
-  Val.orl (Val.andl prev (Val.notl mask))
-          (Val.andl (Val.shll fld (Vint (Int.repr start))) mask).
+  if is_bitfieldl stop start
+  then
+    Val.orl (Val.andl prev (Val.notl mask))
+            (Val.andl (Val.shll fld (Vint (Int.repr start))) mask)
+  else Vundef.
